LiveVerif/src/LiveVerifExamples/Tests/test_PredicateSize_not_found.v
@@ -1,0 +1,43 @@
+(* -*- eval: (load-file "../../LiveVerif/live_verif_setup.el"); -*- *)
+Require Import LiveVerif.LiveVerifLib.
+
+Load LiveVerif.
+
+Context (my_pred1 my_pred2: word -> mem -> Prop).
+
+#[export] Instance spec_of_test: fnspec :=                                      .**/
+
+void test(uintptr_t p, uintptr_t q) /**#
+  ghost_args := (R: mem -> Prop);
+  requires t m := <{ * my_pred1 p
+                     * my_pred2 q
+                     * R }> m;
+  ensures t' m' := t' = t /\
+            <{ * my_pred1 p
+               * my_pred2 q
+               * R }> m' #**/                                              /**.
+Derive test SuchThat (fun_correct! test) As test_ok.                            .**/
+{                                                                          /**.
+  lazymatch goal with
+  | _: message_scope_marker (cannot_purify (my_pred1 p)) |- _ => idtac
+  end.
+  lazymatch goal with
+  | _: message_scope_marker (cannot_purify (my_pred2 q)) |- _ => idtac
+  end.
+
+  (* Test: should not loop infinitely: *)
+  .**/ uintptr_t a = load(p); /**.
+
+  lazymatch goal with
+  | _: message_scope_marker (PredicateSize_not_found my_pred1) |- _ => idtac
+  end.
+  lazymatch goal with
+  | _: message_scope_marker (PredicateSize_not_found my_pred2) |- _ => idtac
+  end.
+
+  test_error Error:("Exactly one of the following subrange claims should hold:" nil).
+Abort.
+
+End LiveVerif.
+
+Comments .**/ //.
